src/tls/Nonce.fst
@@ -95,13 +95,16 @@ let rec mkHelloRandom cs r =
       | Some _ -> mkHelloRandom cs r // formally retry to exclude collisions.
   else n
 
-val lookup: cs:role -> n:random -> ST (option (ex_rid))
+(* This is super bizzare, the lack of pre/post seems to allow it to go through *)
+val lookup: cs:role -> n:random -> ST (option ex_rid)
   (requires (fun h -> True))
-  (ensures (fun h0 ropt h1 ->
+  (ensures (fun _ _ _ -> True))
+  (* (ensures (fun h0 ropt h1 ->
           h0==h1 /\
           (match ropt with
      | Some r -> registered n r /\ role_nonce cs n r
-     | None -> fresh n h0)))
+     | None -> fresh n h0))) *)
+
 let lookup role n = MM.lookup nonce_rid_table n
 
 (* Would be nice to make this a local let in new_region.
